proof/NoDup.v
@@ -4,32 +4,60 @@ From Coq Require Import Lists.List.
 From Coq Require Import Strings.String.
 From PLF Require Import RfTypeDef.
 From PLF Require Import LinearContext.
+From PLF Require Import Nstate.
+
 Import ListNotations.
+Import Nstate.
 
 Definition lcontxt := linear_context overunderty.
 
-Inductive type_ctx_no_dup: lcontxt -> Prop :=
-| type_ctx_no_dup_nil: type_ctx_no_dup nil
-| type_ctx_no_dup_cons: forall x tau_x Gamma,
+Inductive type_ctx_no_dup: tystate -> lcontxt -> Prop :=
+| type_ctx_no_dup_nil: forall tyst, type_ctx_no_dup tyst nil
+| type_ctx_no_dup_cons: forall tyst x tau_x Gamma,
+    tyst x = None ->
     l_find_right_most Gamma x = None ->
-    type_ctx_no_dup ((x, tau_x) :: Gamma).
+    type_ctx_no_dup tyst ((x, tau_x) :: Gamma).
 
 Global Hint Constructors type_ctx_no_dup: core.
 
-Lemma type_ctx_no_dup_cannot_find_last: forall Gamma b tau_b,
-    type_ctx_no_dup (Gamma ++ ((b, tau_b)::nil)) -> l_find_right_most Gamma b = None.
+Lemma type_ctx_no_dup_cannot_find_fst: forall tyst Gamma b tau_b,
+    type_ctx_no_dup tyst ((b, tau_b)::Gamma) -> l_find_right_most Gamma b = None.
+Proof. intros. inversion H. auto. Qed.
+
+Global Hint Resolve type_ctx_no_dup_cannot_find_fst: core.
+
+Lemma type_ctx_no_dup_cannot_find_fst_in_nst: forall tyst Gamma b tau_b,
+    type_ctx_no_dup tyst ((b, tau_b)::Gamma) -> tyst b = None.
+Proof. intros. inversion H. auto. Qed.
+
+Global Hint Resolve type_ctx_no_dup_cannot_find_fst_in_nst: core.
+
+Lemma type_ctx_no_dup_cannot_find_last: forall tyst Gamma b tau_b,
+    type_ctx_no_dup tyst (Gamma ++ ((b, tau_b)::nil)) -> l_find_right_most Gamma b = None.
 Admitted.
 
 Global Hint Resolve type_ctx_no_dup_cannot_find_last: core.
 
-Lemma type_ctx_no_dup_fst_last_diff_name: forall a tau_a Gamma b tau_b,
-    type_ctx_no_dup ((a, tau_a)::Gamma ++ ((b, tau_b)::nil)) -> a <> b.
+Lemma type_ctx_no_dup_cannot_find_last_in_nst: forall tyst Gamma b tau_b,
+    type_ctx_no_dup tyst (Gamma ++ ((b, tau_b)::nil)) -> tyst b = None.
+Admitted.
+
+Global Hint Resolve type_ctx_no_dup_cannot_find_last_in_nst: core.
+
+Lemma type_ctx_no_dup_fst_last_diff_name: forall tyst a tau_a Gamma b tau_b,
+    type_ctx_no_dup tyst ((a, tau_a)::Gamma ++ ((b, tau_b)::nil)) -> a <> b.
 Admitted.
 
 Global Hint Resolve type_ctx_no_dup_fst_last_diff_name: core.
 
-Lemma type_ctx_no_dup_ctx_sub: forall Gamma1 Gamma2,
-    type_ctx_no_dup (Gamma1 ++ Gamma2) -> type_ctx_no_dup Gamma1 /\ type_ctx_no_dup Gamma2.
+Lemma type_ctx_no_dup_ctx_pre: forall tyst Gamma1 Gamma2,
+    type_ctx_no_dup tyst (Gamma1 ++ Gamma2) -> type_ctx_no_dup tyst Gamma1.
 Admitted.
 
-Global Hint Resolve type_ctx_no_dup_ctx_sub: core.
+Global Hint Resolve type_ctx_no_dup_ctx_pre: core.
+
+Lemma type_ctx_no_dup_ctx_post: forall tyst Gamma1 Gamma2,
+    type_ctx_no_dup tyst (Gamma1 ++ Gamma2) -> type_ctx_no_dup tyst Gamma2.
+Admitted.
+
+Global Hint Resolve type_ctx_no_dup_ctx_post: core.
