proof/NormalTypeSystemSimp.v
@@ -4,17 +4,17 @@ From PLF Require Import Types.
 From PLF Require Import Smallstep.
 From PLF Require Import CoreLangSimp.
 
-Ltac invert :=
-  match goal with | H : ?T |- _ =>
-                      match type of T with Prop => solve [exfalso; apply H; auto]
-                      end
-  end.
+(* Ltac invert := *)
+(*   match goal with | H : ?T \N- _ => *)
+(*                       match type of T with Prop => solve [exfalso; apply H; auto] *)
+(*                       end *)
+(*   end. *)
 
 Import CoreLangSimp.
 
 Definition context := partial_map ty.
 
-Reserved Notation "Gamma '|-' t '\Tin' T" (at level 40).
+Reserved Notation "Gamma '\N-' t '\Tin' T" (at level 40).
 
 Inductive has_type : context -> tm -> ty -> Prop :=
 | T_Exn : forall Gamma T, has_type Gamma texn T
@@ -47,21 +47,21 @@ with value_has_type : context -> value -> ty -> Prop :=
     has_type (update Gamma x T11) t12 T12 ->
     value_has_type Gamma (vlam x T11 t12) (TArrow T11 T12)
 
-where "Gamma '|-' t '\Tin' T" := (has_type Gamma t T).
-Notation "Gamma '|-' t '\Vin' T" := (value_has_type Gamma t T) (at level 40).
+where "Gamma '\N-' t '\Tin' T" := (has_type Gamma t T).
+Notation "Gamma '\N-' t '\Vin' T" := (value_has_type Gamma t T) (at level 40).
 
 Global Hint Constructors has_type: core.
 Global Hint Constructors value_has_type: core.
 
-Lemma empty_has_type_implies_closed: forall e T, empty |- e \Tin T -> (forall x, ~ x \FVtm e).
+Lemma empty_has_type_implies_closed: forall e T, empty \N- e \Tin T -> (forall x, ~ x \FVtm e).
 Admitted.
 
 Global Hint Resolve empty_has_type_implies_closed: core.
 
 Lemma eval_op_is_type_safe: forall Gamma op (c1 c2 c3: constant) (T1 T2 T3: base_ty),
-    Gamma |- c1 \Vin T1 -> Gamma |- c2 \Vin T2 ->
+    Gamma \N- c1 \Vin T1 -> Gamma \N- c2 \Vin T2 ->
                                  eval_op op c1 c2 c3 -> ty_of_op op = T1 t--> (T2 t--> T3) ->
-                                 empty |- c3 \Vin T3.
+                                 empty \N- c3 \Vin T3.
 Proof.
   intros Gamma op c1 c2 c3 T1 T2 T3 Hc1 Hc2 Heval Hop.
   destruct Heval; inversion Hc1; subst; inversion Hc2; subst; inversion Hop; subst; constructor.
@@ -70,7 +70,7 @@ Qed.
 Global Hint Resolve eval_op_is_type_safe: core.
 
 Lemma base_value_const_exists:
-  forall T v, empty |- v \Vin (TBase T) -> (exists c, v = vconst c).
+  forall T v, empty \N- v \Vin (TBase T) -> (exists c, v = vconst c).
 Proof.
   intros.
   destruct v; inversion H; subst; eauto.
@@ -79,21 +79,21 @@ Qed.
 
 Global Hint Resolve base_value_const_exists: core.
 
-Lemma nat_const_n_exists: forall Gamma (c: constant), Gamma |- c \Vin (TBase TNat) -> (exists (n: nat), c = n).
+Lemma nat_const_n_exists: forall Gamma (c: constant), Gamma \N- c \Vin (TBase TNat) -> (exists (n: nat), c = n).
 Proof with eauto.
   intros. destruct c; inversion H; subst...
 Qed.
 
 Global Hint Resolve nat_const_n_exists: core.
 
-Lemma bool_const_b_exists: forall Gamma (c: constant), Gamma |- c \Vin (TBase TBool) -> (exists (n: bool), c = n).
+Lemma bool_const_b_exists: forall Gamma (c: constant), Gamma \N- c \Vin (TBase TBool) -> (exists (n: bool), c = n).
 Proof with eauto.
   intros. destruct c; inversion H; subst...
 Qed.
 
 Global Hint Resolve bool_const_b_exists: core.
 
-Lemma nat_value_n_exists: forall v, empty |- v \Vin (TBase TNat) -> (exists n, v = (vconst (cnat n))).
+Lemma nat_value_n_exists: forall v, empty \N- v \Vin (TBase TNat) -> (exists n, v = (vconst (cnat n))).
 Proof with eauto.
   intros. assert (exists c, v = vconst c) as HH...
   destruct HH as (c & Hc); subst... eapply nat_const_n_exists in H... destruct H; subst...
@@ -101,7 +101,7 @@ Qed.
 
 Global Hint Resolve nat_value_n_exists: core.
 
-Lemma bool_value_b_exists: forall v, empty |- v \Vin (TBase TBool) -> (exists b, v = (vconst (cbool b))).
+Lemma bool_value_b_exists: forall v, empty \N- v \Vin (TBase TBool) -> (exists b, v = (vconst (cbool b))).
 Proof with eauto.
   intros. assert (exists c, v = vconst c) as HH...
   destruct HH as (c & Hc); subst... eapply bool_const_b_exists in H... destruct H; subst...
@@ -110,7 +110,7 @@ Qed.
 Global Hint Resolve bool_value_b_exists: core.
 
 Lemma base_value_cid_exists:
-  forall Gamma T v, Gamma |- v \Vin (TBase T) -> ((exists c, v = vconst c) \/ (exists (name: string), v = name)).
+  forall Gamma T v, Gamma \N- v \Vin (TBase T) -> ((exists c, v = vconst c) \/ (exists (name: string), v = name)).
 Proof.
   intros.
   destruct v.
@@ -121,7 +121,7 @@ Qed.
 
 Global Hint Resolve base_value_cid_exists: core.
 
-Lemma nat_value_cid_exists: forall Gamma v, Gamma |- v \Vin (TBase TNat) ->
+Lemma nat_value_cid_exists: forall Gamma v, Gamma \N- v \Vin (TBase TNat) ->
                                                ((exists n, v = (vconst (cnat n))) \/ (exists (name: string), v = name)).
 Proof with eauto.
   intros. assert ((exists c : constant, v = c) \/ (exists name : string, v = name)) as HH... destruct HH.
@@ -129,7 +129,7 @@ Proof with eauto.
   - right. destruct H0; subst...
 Qed.
 
-Lemma bool_value_cid_exists: forall Gamma v, Gamma |- v \Vin (TBase TBool) ->
+Lemma bool_value_cid_exists: forall Gamma v, Gamma \N- v \Vin (TBase TBool) ->
                                                ((exists n, v = (vconst (cbool n))) \/ (exists (name: string), v = name)).
 Proof with eauto.
   intros. assert ((exists c : constant, v = c) \/ (exists name : string, v = name)) as HH... destruct HH.
@@ -138,7 +138,7 @@ Proof with eauto.
 Qed.
 
 (* Lemma arrow_value_lam_exists: forall v T1 T2, *)
-(*     empty |- v \Vin (TArrow T1 T2) -> exists x e, v = vlam x T1 e. *)
+(*     empty \N- v \Vin (TArrow T1 T2) -> exists x e, v = vlam x T1 e. *)
 (* Proof. *)
 (*   intros. *)
 (*   destruct v; inversion H; subst; eauto. *)
@@ -146,7 +146,7 @@ Qed.
 (*   - inversion H2. *)
 (* Qed. *)
 
-Lemma has_type_inv_value: forall Gamma v T, Gamma |- tvalue v \Tin T -> Gamma |- v \Vin T.
+Lemma has_type_inv_value: forall Gamma v T, Gamma \N- tvalue v \Tin T -> Gamma \N- v \Vin T.
 Proof.
   intros.
   inversion H; subst; auto.
@@ -161,12 +161,12 @@ Qed.
 
 Lemma weakening : forall e T Gamma Gamma',
     includedin Gamma Gamma' ->
-    (Gamma  |- e \Tin T -> Gamma' |- e \Tin T).
+    (Gamma  \N- e \Tin T -> Gamma' \N- e \Tin T).
 Proof.
   intro e.
   apply (tm_mutual_rec
-         (fun v => forall T Gamma Gamma', includedin Gamma Gamma' -> (Gamma  |- v \Vin T -> Gamma' |- v \Vin T))
-         (fun e => forall T Gamma Gamma', includedin Gamma Gamma' -> (Gamma  |- e \Tin T -> Gamma' |- e \Tin T))).
+         (fun v => forall T Gamma Gamma', includedin Gamma Gamma' -> (Gamma  \N- v \Vin T -> Gamma' \N- v \Vin T))
+         (fun e => forall T Gamma Gamma', includedin Gamma Gamma' -> (Gamma  \N- e \Tin T -> Gamma' \N- e \Tin T))).
   - intros; inversion H0; subst; eauto 7 using includedin_update.
   - intros; inversion H0; subst; eauto 7 using includedin_update.
   - intros; inversion H1; subst; eauto 7 using includedin_update.
@@ -181,7 +181,7 @@ Qed.
 
 Lemma value_weakening : forall e T Gamma Gamma',
     includedin Gamma Gamma' ->
-    (Gamma  |- e \Vin T -> Gamma' |- e \Vin T).
+    (Gamma  \N- e \Vin T -> Gamma' \N- e \Vin T).
 Proof.
   intros.
   apply weakening with (e:=tvalue e) (T:=T) in H; auto.
@@ -189,7 +189,7 @@ Proof.
 Qed.
 
 Lemma weakening_empty : forall Gamma t T,
-    empty |- t \Tin T  -> Gamma |- t \Tin T.
+    empty \N- t \Tin T  -> Gamma \N- t \Tin T.
 Proof.
   intros Gamma t T.
   eapply weakening.
@@ -197,16 +197,16 @@ Proof.
 Qed.
 
 Lemma value_weakening_empty : forall Gamma t T,
-    empty |- t \Vin T  -> Gamma |- t \Vin T.
+    empty \N- t \Vin T  -> Gamma \N- t \Vin T.
 Proof.
   intros Gamma t T H.
-  assert (empty |- (tvalue t) \Tin T). auto.
+  assert (empty \N- (tvalue t) \Tin T). auto.
   apply weakening_empty with (Gamma:=Gamma) in H0. inversion H0; subst; auto.
 Qed.
 
 Lemma substitution_preserves_typing2:
   (forall (s : string) (Gamma : partial_map ty) (x : string) (U : ty) (v : value) (T : ty),
-      (x |-> U; Gamma) |- s \Vin T -> empty |- v \Vin U -> Gamma |- [x := v ]v s \Vin T).
+      (x |-> U; Gamma) \N- s \Vin T -> empty \N- v \Vin U -> Gamma \N- [x := v ]v s \Vin T).
 Proof.
   intros. inversion H; clear H; subst; simpl; eauto.
   rename s into y. rename x into x.
@@ -222,12 +222,12 @@ Qed.
 Lemma substitution_preserves_typing7:
   (forall (s : string) (t : tm),
       (forall (Gamma : partial_map ty) (x : string) (U : ty) (v : value) (T : ty),
-          (x |-> U; Gamma) |- t \Tin T -> empty |- v \Vin U -> Gamma |- [x := v] t \Tin T) ->
+          (x |-> U; Gamma) \N- t \Tin T -> empty \N- v \Vin U -> Gamma \N- [x := v] t \Tin T) ->
       forall t0 : tm,
         (forall (Gamma : partial_map ty) (x : string) (U : ty) (v : value) (T : ty),
-            (x |-> U; Gamma) |- t0 \Tin T -> empty |- v \Vin U -> Gamma |- [x := v] t0 \Tin T) ->
+            (x |-> U; Gamma) \N- t0 \Tin T -> empty \N- v \Vin U -> Gamma \N- [x := v] t0 \Tin T) ->
         forall (Gamma : partial_map ty) (x : string) (U : ty) (v : value) (T : ty),
-          (x |-> U; Gamma) |- tlete s t t0 \Tin T -> empty |- v \Vin U -> Gamma |- [x := v] tlete s t t0 \Tin T).
+          (x |-> U; Gamma) \N- tlete s t t0 \Tin T -> empty \N- v \Vin U -> Gamma \N- [x := v] tlete s t t0 \Tin T).
 Proof.
   intros. inversion H1; clear H1; subst; simpl; eauto.
   rename s into y. rename x into x.
@@ -243,15 +243,15 @@ Qed.
 Lemma substitution_preserves_typing9:
   (forall (s : string) (v : value),
       (forall (Gamma : partial_map ty) (x : string) (U : ty) (v0 : value) (T : ty),
-          (x |-> U; Gamma) |- v \Vin T -> empty |- v0 \Vin U -> Gamma |- [x := v0 ]v v \Vin T) ->
+          (x |-> U; Gamma) \N- v \Vin T -> empty \N- v0 \Vin U -> Gamma \N- [x := v0 ]v v \Vin T) ->
       forall v0 : value,
         (forall (Gamma : partial_map ty) (x : string) (U : ty) (v1 : value) (T : ty),
-            (x |-> U; Gamma) |- v0 \Vin T -> empty |- v1 \Vin U -> Gamma |- [x := v1 ]v v0 \Vin T) ->
+            (x |-> U; Gamma) \N- v0 \Vin T -> empty \N- v1 \Vin U -> Gamma \N- [x := v1 ]v v0 \Vin T) ->
         forall t : tm,
           (forall (Gamma : partial_map ty) (x : string) (U : ty) (v1 : value) (T : ty),
-              (x |-> U; Gamma) |- t \Tin T -> empty |- v1 \Vin U -> Gamma |- [x := v1] t \Tin T) ->
+              (x |-> U; Gamma) \N- t \Tin T -> empty \N- v1 \Vin U -> Gamma \N- [x := v1] t \Tin T) ->
           forall (Gamma : partial_map ty) (x : string) (U : ty) (v1 : value) (T : ty),
-            (x |-> U; Gamma) |- tletapp s v v0 t \Tin T -> empty |- v1 \Vin U -> Gamma |- [x := v1] tletapp s v v0 t \Tin T).
+            (x |-> U; Gamma) \N- tletapp s v v0 t \Tin T -> empty \N- v1 \Vin U -> Gamma \N- [x := v1] tletapp s v v0 t \Tin T).
 Proof.
   intros. inversion H2; clear H2; subst; simpl; eauto.
   rename s into y. rename x into x.
@@ -268,12 +268,12 @@ Proof.
 Qed.
 
 Lemma substitution_preserves_typing : forall t Gamma x U v T,
-    (x |-> U ; Gamma) |- t \Tin T ->  empty |- v \Vin U  ->  Gamma |- [x:=v]t \Tin T.
+    (x |-> U ; Gamma) \N- t \Tin T ->  empty \N- v \Vin U  ->  Gamma \N- [x:=v]t \Tin T.
 Proof with eauto.
   intro t.
   apply (tm_mutual_rec
-           (fun ev => forall Gamma x U v T, (x |-> U ; Gamma) |- ev \Vin T ->  empty |- v \Vin U ->  Gamma |- [x:=v]v ev \Vin T)
-           (fun e => forall Gamma x U v T, (x |-> U ; Gamma) |- e \Tin T ->  empty |- v \Vin U ->  Gamma |- [x:=v] e \Tin T)).
+           (fun ev => forall Gamma x U v T, (x |-> U ; Gamma) \N- ev \Vin T ->  empty \N- v \Vin U ->  Gamma \N- [x:=v]v ev \Vin T)
+           (fun e => forall Gamma x U v T, (x |-> U ; Gamma) \N- e \Tin T ->  empty \N- v \Vin U ->  Gamma \N- [x:=v] e \Tin T)).
   - intro c. induction c; intros; inversion H; clear H; subst; simpl; eauto; constructor...
   - intro c. destruct c.
     + intros. inversion H; clear H; subst; simpl; eauto; constructor...
@@ -296,9 +296,9 @@ Proof with eauto.
 Qed.
 
 Theorem preservation : forall t t' T,
-    empty |- t \Tin T  ->
+    empty \N- t \Tin T  ->
                   t --> t'  ->
-                  empty |- t' \Tin T.
+                  empty \N- t' \Tin T.
 Proof with eauto.
   intros t t' T HT. generalize dependent t'.
   remember empty as Gamma.
@@ -313,12 +313,18 @@ Proof with eauto.
 Qed.
 
 Theorem preservation_value : forall t (v: value) T,
-    empty |- t \Tin T  -> t -->* v  ->
-                  empty |- v \Vin T.
+    empty \N- t \Tin T  -> t -->* v  ->
+                  empty \N- v \Vin T.
 Proof.
 Admitted.
 
-(* Definition any_ctx_const_nat_typed_is_nat: forall Gamma (c: constant), Gamma |- c \Vin TNat -> exists (n: nat), c = n. *)
+Theorem const_ctx_independent : forall Gamma (c:constant) T,
+    Gamma \N- c \Tin T <-> empty \N- c \Tin T.
+Proof.
+Admitted.
+
+
+(* Definition any_ctx_const_nat_typed_is_nat: forall Gamma (c: constant), Gamma \N- c \Vin TNat -> exists (n: nat), c = n. *)
 (* Proof with eauto. *)
 (*   intros. inversion H; subst. exists n... *)
 (* Qed. *)
